refactor: decouple the wrapper from the C opsem
Instead, define a separate notion of "C interface" that only defines C
values and the C heap. (Conceptually, this is "the C ABI".) The
wrapper then only depends on the C interface, and is able to
interoperate with any language that implements this C interface.

theories/c_lang/lang.v
@@ -4,15 +4,13 @@ From iris.algebra Require Export ofe.
 From iris.heap_lang Require Export locations.
 From iris.prelude Require Import options.
 From melocoton Require Import commons.
+From melocoton.c_interface Require Import defs.
 
 Declare Scope expr_scope.
-Declare Scope val_scope.
 Delimit Scope expr_scope with E.
-Delimit Scope val_scope with V.
 
 Module C_lang.
-Inductive base_lit : Set :=
-  | LitInt (n : Z) | LitLoc (l : loc) | LitFunPtr (x : string).
+
 Inductive un_op : Set :=
   | NegOp | NotOp | BitwiseNotOp | Ptr2Int | Int2Ptr .
 Inductive bin_op : Set :=
@@ -24,9 +22,6 @@ Inductive bin_op : Set :=
   | ShiftLOp | ShiftROp (* Shifts *)
   | LeOp | LtOp | EqOp (* Relations *)
   | PtrOffsetOp | PtrDiffOp.
-
-Inductive val :=
-  | LitV (l : base_lit).
 
 Unset Elimination Schemes.
 Inductive expr :=
@@ -186,7 +181,6 @@ Proof.
 Defined.
 
 Bind Scope expr_scope with expr.
-Bind Scope val_scope with val.
 
 Inductive function := Fun (b : list binder) (e : expr).
 
@@ -223,13 +217,9 @@ Local Notation to_val e :=
 Global Instance of_val_inj : Inj (=) (=) of_val.
 Proof. intros ??. congruence. Qed.
 
-Global Instance base_lit_eq_dec : EqDecision base_lit.
-Proof. solve_decision. Defined.
 Global Instance un_op_eq_dec : EqDecision un_op.
 Proof. solve_decision. Defined.
 Global Instance bin_op_eq_dec : EqDecision bin_op.
-Proof. solve_decision. Defined.
-Global Instance val_eq_dec : EqDecision val.
 Proof. solve_decision. Defined.
 Global Instance expr_eq_dec : EqDecision expr.
 Proof.
@@ -263,29 +253,9 @@ Proof.
      end); try (clear gol); (clear go; abstract intuition congruence).
 Defined.
 
-Notation heap_cell := (option (option val)).
-Notation Deallocated := (None : heap_cell).
-Notation Uninitialized := (Some None : heap_cell).
-Notation Storing v := (Some (Some v) : heap_cell).
-
-(** The state: heaps of heap_cells. *)
-Local Notation state := (gmap loc heap_cell).
-
 Class program := prog : gmap string function.
 
 
-Global Instance base_lit_countable : Countable base_lit.
-Proof.
- refine (inj_countable' (λ l, match l with
-  | LitInt n => (inl (inl n))
-  | LitLoc l => (inl (inr l))
-  | LitFunPtr p => (inr p)
-  end) (λ l, match l with
-  | inl (inl n) => LitInt n
-  | inl (inr l) => LitLoc l
-  | inr p => LitFunPtr p
-  end) _); by intros [].
-Qed.
 Global Instance un_op_finite : Countable un_op.
 Proof.
  refine (inj_countable' (λ op, match op with NegOp => 0 | NotOp => 1 | BitwiseNotOp => 2 | Ptr2Int => 3 | Int2Ptr => 4 end)
@@ -302,13 +272,6 @@ Proof.
   | 5 => AndOp | 6 => OrOp | 7 => XorOp | 8 => ShiftLOp | 9 => ShiftROp
   | 10 => LeOp | 11 => LtOp | 12 => EqOp | 13 => PtrOffsetOp | _ => PtrDiffOp
   end) _); by intros [].
-Qed.
-Global Instance val_countable : Countable val.
-Proof. 
-  set (enc := fun e => match e with LitV l => l end).
-  set (dec := LitV).
-  refine (inj_countable' enc dec _).
-  by intros [].
 Qed.
 
 Global Instance expr_countable : Countable expr.
@@ -353,15 +316,9 @@ Proof. (* string + binder + un_op + bin_op + val *)
  all: unfold map; by induction ee as [|ex er ->]; simpl; f_equal.
 Qed.
 
-
-Global Instance state_inhabited : Inhabited state :=
-  populate inhabitant.
-Global Instance val_inhabited : Inhabited val := populate (LitV (LitInt 0)).
 Global Instance expr_inhabited : Inhabited expr := populate (Val inhabitant).
 
-Canonical Structure stateO := leibnizO state.
 Canonical Structure locO := leibnizO loc.
-Canonical Structure valO := leibnizO val.
 Canonical Structure exprO := leibnizO expr.
 
 (** Evaluation contexts *)
@@ -440,9 +397,6 @@ Definition un_op_eval (op : un_op) (v : val) : option val :=
   | _, _ => None
   end.
 
-Definition LitBool (b : bool) : base_lit := LitInt (if b then 1%Z else 0%Z).
-Definition LitUnit : base_lit := LitInt 0.
-
 Definition bin_op_eval (op : bin_op) (v1 v2 : val) : option base_lit :=
   match op, v1, v2 with
   | PlusOp, LitV (LitInt n1), LitV (LitInt n2) => Some $ LitInt (n1 + n2)
@@ -474,51 +428,8 @@ Definition bin_op_eval (op : bin_op) (v1 v2 : val) : option base_lit :=
   | LitFunPtr _, LitFunPtr _ => True
   | _,_ => False end.
 
-Definition state_upd_heap (f: gmap loc heap_cell → gmap loc heap_cell) (σ: state) : state :=
-  f σ.
-Global Arguments state_upd_heap _ !_ /.
-
-Fixpoint heap_array (l : loc) (vs : list heap_cell) : gmap loc heap_cell :=
-  match vs with
-  | [] => ∅
-  | v :: vs' => {[l := v]} ∪ heap_array (l +ₗ 1) vs'
-  end.
-
-Lemma heap_array_singleton l v : heap_array l [v] = {[l := v]}.
-Proof. by rewrite /heap_array right_id. Qed.
-
-Lemma heap_array_lookup l vs ow k :
-  heap_array l vs !! k = Some ow ↔
-  ∃ j, (0 ≤ j)%Z ∧ k = l +ₗ j ∧ vs !! (Z.to_nat j) = Some ow.
-Proof.
-  revert k l; induction vs as [|v' vs IH]=> l' l /=.
-  { rewrite lookup_empty. naive_solver lia. }
-  rewrite -insert_union_singleton_l lookup_insert_Some IH. split.
-  - intros [[-> ?] | (Hl & j  & ? & -> & ?)].
-    { eexists 0. rewrite loc_add_0. naive_solver lia. }
-    eexists (1 + j)%Z. rewrite loc_add_assoc !Z.add_1_l Z2Nat.inj_succ; auto with lia.
-  - intros (j & w & -> & Hil). destruct (decide (j = 0)); simplify_eq/=.
-    { rewrite loc_add_0; eauto. }
-    right. split.
-    { rewrite -{1}(loc_add_0 l). intros ?%(inj (loc_add _)); lia. }
-    assert (Z.to_nat j = S (Z.to_nat (j - 1))) as Hj.
-    { rewrite -Z2Nat.inj_succ; last lia. f_equal; lia. }
-    rewrite Hj /= in Hil.
-    eexists (j - 1)%Z. rewrite loc_add_assoc Z.add_sub_assoc Z.add_simpl_l.
-    auto with lia.
-Qed.
-
-Lemma heap_array_map_disjoint (h : gmap loc heap_cell) (l : loc) (vs : list _) :
-  (∀ i, (0 ≤ i)%Z → (i < length vs)%Z → h !! (l +ₗ i) = None) →
-  (heap_array l vs) ##ₘ h.
-Proof.
-  intros Hdisj. apply map_disjoint_spec=> l' v1 v2.
-  intros (j&w&->&Hj%lookup_lt_Some%inj_lt)%heap_array_lookup.
-  move: Hj. rewrite Z2Nat.id // => ?. by rewrite Hdisj.
-Qed.
-
 (* [h] is added on the right here to make [state_init_heap_singleton] true. *)
-Definition state_init_heap (l : loc) (n : Z) (v : heap_cell) (σ : state) : state :=
+Definition state_init_heap (l : loc) (n : Z) (v : heap_cell) (σ : c_state) : c_state :=
   state_upd_heap (λ h, heap_array l (replicate (Z.to_nat n) v) ∪ h) σ.
 
 Lemma state_init_heap_singleton l v σ :
@@ -545,7 +456,7 @@ Fixpoint zip_args (an : list binder) (av : list val) : option (gmap string val) 
 Definition apply_function (f:function) (av : list val) := match f with Fun an e =>
     match (zip_args an av) with Some σ => Some (subst_all σ e) | _ => None end end.
 
-Inductive head_step (p : program) : expr → state → expr → state → Prop :=
+Inductive head_step (p : program) : expr → c_state → expr → c_state → Prop :=
   | LetS x v1 e2 ee σ :
      ee = subst' x v1 e2 ->
      head_step p (Let x (Val v1) e2) σ ee σ
