theories/c_lang/primitive_laws.v
@@ -3,131 +3,17 @@ the Iris lifting lemmas. *)
 
 From iris.proofmode Require Import proofmode.
 From iris.bi.lib Require Import fractional.
-From iris.base_logic.lib Require Import mono_nat.
 From iris.base_logic.lib Require Export gen_heap proph_map gen_inv_heap.
 From melocoton.language Require Export weakestpre lifting.
+From melocoton.c_interface Require Export resources.
 From melocoton.c_lang Require Export class_instances.
 From melocoton.c_lang Require Import tactics notation.
 From iris.prelude Require Import options.
-
-Class heapGS_C Σ := HeapGS {
-  heapGS_gen_heapGS :> gen_heapGS loc heap_cell Σ;
-  heapGS_inv_heapGS :> inv_heapGS loc heap_cell Σ;
-  heapGS_proph_mapGS :> proph_mapGS positive (prod val val) Σ;
-  heapGS_step_name : gname;
-  heapGS_step_cnt : mono_natG Σ;
-}.
-Local Existing Instance heapGS_step_cnt.
-
-Section steps.
-  Context `{!heapGS_C Σ}.
-
-  Local Definition steps_auth (n : nat) : iProp Σ :=
-    mono_nat_auth_own heapGS_step_name 1 n.
-
-  Definition steps_lb (n : nat) : iProp Σ :=
-    mono_nat_lb_own heapGS_step_name n.
-
-  Local Lemma steps_lb_valid n m :
-    steps_auth n -∗ steps_lb m -∗ ⌜m ≤ n⌝.
-  Proof.
-    iIntros "Hauth Hlb".
-    by iDestruct (mono_nat_lb_own_valid with "Hauth Hlb") as %[_ Hle].
-  Qed.
-
-  Local Lemma steps_lb_get n :
-    steps_auth n -∗ steps_lb n.
-  Proof. apply mono_nat_lb_own_get. Qed.
-
-  Local Lemma steps_auth_update n n' :
-    n ≤ n' → steps_auth n ==∗ steps_auth n' ∗ steps_lb n'.
-  Proof. intros Hle. by apply mono_nat_own_update. Qed.
-
-  Local Lemma steps_auth_update_S n :
-    steps_auth n ==∗ steps_auth (S n).
-  Proof.
-    iIntros "Hauth".
-    iMod (mono_nat_own_update with "Hauth") as "[$ _]"; [lia|done].
-  Qed.
-
-  Lemma steps_lb_le n n' :
-    n' ≤ n → steps_lb n -∗ steps_lb n'.
-  Proof. intros Hle. by apply mono_nat_lb_own_le. Qed.
-
-End steps.
 
 Global Program Instance heapGS_langGS_C `{heapGS_C Σ}
       : langGS val C_lang Σ := {
   state_interp σ := gen_heap_interp σ
 }.
-
-(** Since we use an [option val] instance of [gen_heap], we need to overwrite
-the notations.  That also helps for scopes and coercions. *)
-(** FIXME: Refactor these notations using custom entries once Coq bug #13654
-has been fixed. *)
-
-Notation "l O↦{ dq } v" := (mapsto (L:=loc) (V:=heap_cell) l dq (v))
-  (at level 20, format "l  O↦{ dq }  v") : bi_scope.
-Notation "l O↦□ v" := (mapsto (L:=loc) (V:=heap_cell) l DfracDiscarded (v))
-  (at level 20, format "l  O↦□  v") : bi_scope.
-Notation "l O↦{# q } v" := (mapsto (L:=loc) (V:=heap_cell) l (DfracOwn q) (v))
-  (at level 20, format "l  O↦{# q }  v") : bi_scope.
-Notation "l O↦ v" := (mapsto (L:=loc) (V:=heap_cell) l (DfracOwn 1) (v))
-  (at level 20, format "l  O↦  v") : bi_scope.
-
-Notation "l I↦{ dq } v" := (mapsto (L:=loc) (V:=heap_cell) l dq (Some v))
-  (at level 20, format "l  I↦{ dq }  v") : bi_scope.
-Notation "l I↦□ v" := (mapsto (L:=loc) (V:=heap_cell) l DfracDiscarded (Some v))
-  (at level 20, format "l  I↦□  v") : bi_scope.
-Notation "l I↦{# q } v" := (mapsto (L:=loc) (V:=heap_cell) l (DfracOwn q) (Some v))
-  (at level 20, format "l  I↦{# q }  v") : bi_scope.
-Notation "l I↦ v" := (mapsto (L:=loc) (V:=heap_cell) l (DfracOwn 1) (Some v))
-  (at level 20, format "l  I↦  v") : bi_scope.
-
-Notation "l ↦C{ dq } v" := (mapsto (L:=loc) (V:=heap_cell) l dq (Some (Some v%V)))
-  (at level 20, format "l  ↦C{ dq }  v") : bi_scope.
-Notation "l ↦C□ v" := (mapsto (L:=loc) (V:=heap_cell) l DfracDiscarded (Storing v%V))
-  (at level 20, format "l  ↦C□  v") : bi_scope.
-Notation "l ↦C{# q } v" := (mapsto (L:=loc) (V:=heap_cell) l (DfracOwn q) (Storing v%V))
-  (at level 20, format "l  ↦C{# q }  v") : bi_scope.
-Notation "l ↦C v" := (mapsto (L:=loc) (V:=heap_cell) l (DfracOwn 1) (Storing v%V))
-  (at level 20, format "l  ↦C  v") : bi_scope.
-Notation "l ↦C{ dq } '?'" := (mapsto (L:=loc) (V:=heap_cell) l dq (Uninitialized))
-  (at level 20, format "l  ↦C{ dq }  ?") : bi_scope.
-Notation "l ↦C□ '?'" := (mapsto (L:=loc) (V:=heap_cell) l DfracDiscarded (Uninitialized))
-  (at level 20, format "l  ↦C□  ?") : bi_scope.
-Notation "l ↦C{# q } '?'" := (mapsto (L:=loc) (V:=heap_cell) l (DfracOwn q) (Uninitialized))
-  (at level 20, format "l  ↦C{# q }  ?") : bi_scope.
-Notation "l ↦C '?'" := (mapsto (L:=loc) (V:=heap_cell) l (DfracOwn 1) (Uninitialized))
-  (at level 20, format "l  ↦C  ?") : bi_scope.
-
-(** Same for [gen_inv_heap], except that these are higher-order notations so to
-make setoid rewriting in the predicate [I] work we need actual definitions
-here. *)
-Section definitions.
-  Context `{!heapGS_C Σ}.
-
-  Definition from_storing (I : val → Prop) (Puninit Pfree : Prop) (k : heap_cell) :=
-    match k with
-    | None => Pfree
-    | Some None => Puninit
-    | Some (Some v) => I v
-    end.
-
-  Definition inv_mapsto_own (l : loc) (v : val) (I : val → Prop) : iProp Σ :=
-    inv_mapsto_own l (Storing v) (from_storing I False False).
-  Definition inv_mapsto (l : loc) (I : val → Prop) : iProp Σ :=
-    inv_mapsto l (from_storing I False False).
-End definitions.
-
-Global Instance: Params (@inv_mapsto_own) 4 := {}.
-Global Instance: Params (@inv_mapsto) 3 := {}.
-
-Notation inv_heap_inv := (inv_heap_inv loc heap_cell).
-Notation "l '↦_' I □" := (inv_mapsto l I%stdpp%type)
-  (at level 20, I at level 9, format "l  '↦_' I  '□'") : bi_scope.
-Notation "l ↦_ I v" := (inv_mapsto_own l v I%stdpp%type)
-  (at level 20, I at level 9, format "l  ↦_ I  v") : bi_scope.
 
 Section lifting.
 Context `{!heapGS_C Σ, !invGS_gen hlc Σ}.
@@ -160,124 +46,6 @@ Proof.
 Qed.
 
 
-(** Heap *)
-
-(** We need to adjust the [gen_heap] and [gen_inv_heap] lemmas because of our
-value type being [option val]. *)
-
-Lemma mapsto_valid l dq v : l ↦C{dq} v -∗ ⌜✓ dq⌝.
-Proof. apply mapsto_valid. Qed.
-Lemma mapsto_valid_2 l dq1 dq2 v1 v2 :
-  l ↦C{dq1} v1 -∗ l ↦C{dq2} v2 -∗ ⌜✓ (dq1 ⋅ dq2) ∧ v1 = v2⌝.
-Proof.
-  iIntros "H1 H2". iDestruct (mapsto_valid_2 with "H1 H2") as %[? [=?]]. done.
-Qed.
-Lemma mapsto_agree l dq1 dq2 v1 v2 : l ↦C{dq1} v1 -∗ l ↦C{dq2} v2 -∗ ⌜v1 = v2⌝.
-Proof. iIntros "H1 H2". iDestruct (mapsto_agree with "H1 H2") as %[=?]. done. Qed.
-
-Lemma mapsto_combine l dq1 dq2 v1 v2 :
-  l ↦C{dq1} v1 -∗ l ↦C{dq2} v2 -∗ l ↦C{dq1 ⋅ dq2} v1 ∗ ⌜v1 = v2⌝.
-Proof.
-  iIntros "Hl1 Hl2". iDestruct (mapsto_combine with "Hl1 Hl2") as "[$ Heq]".
-  by iDestruct "Heq" as %[= ->].
-Qed.
-
-Lemma mapsto_frac_ne l1 l2 dq1 dq2 v1 v2 :
-  ¬ ✓(dq1 ⋅ dq2) → l1 ↦C{dq1} v1 -∗ l2 ↦C{dq2} v2 -∗ ⌜l1 ≠ l2⌝.
-Proof. apply mapsto_frac_ne. Qed.
-Lemma mapsto_ne l1 l2 dq2 v1 v2 : l1 ↦C v1 -∗ l2 ↦C{dq2} v2 -∗ ⌜l1 ≠ l2⌝.
-Proof. apply mapsto_ne. Qed.
-
-Lemma mapsto_persist l dq v : l ↦C{dq} v ==∗ l ↦C□ v.
-Proof. apply mapsto_persist. Qed.
-
-Global Instance inv_mapsto_own_proper l v :
-  Proper (pointwise_relation _ iff ==> (≡)) (inv_mapsto_own l v).
-Proof.
-  intros I1 I2 HI. rewrite /inv_mapsto_own. f_equiv=>-[[w|]|]; [|done|done].
-  simpl. apply HI.
-Qed.
-Global Instance inv_mapsto_proper l :
-  Proper (pointwise_relation _ iff ==> (≡)) (inv_mapsto l).
-Proof.
-  intros I1 I2 HI. rewrite /inv_mapsto. f_equiv=>-[[w|]|]; [|done|done].
-  simpl. apply HI.
-Qed.
-
-Lemma make_inv_mapsto l v (I : val → Prop) E :
-  ↑inv_heapN ⊆ E →
-  I v →
-  inv_heap_inv -∗ l ↦C v ={E}=∗ l ↦_I v.
-Proof. iIntros (??) "#HI Hl". iApply make_inv_mapsto; done. Qed.
-Lemma inv_mapsto_own_inv l v I : l ↦_I v -∗ l ↦_I □.
-Proof. apply inv_mapsto_own_inv. Qed.
-
-Lemma inv_mapsto_own_acc_strong E :
-  ↑inv_heapN ⊆ E →
-  inv_heap_inv ={E, E ∖ ↑inv_heapN}=∗ ∀ l v I, l ↦_I v -∗
-    (⌜I v⌝ ∗ l ↦C v ∗ (∀ w, ⌜I w ⌝ -∗ l ↦C w ==∗
-      inv_mapsto_own l w I ∗ |={E ∖ ↑inv_heapN, E}=> True)).
-Proof.
-  iIntros (?) "#Hinv".
-  iMod (inv_mapsto_own_acc_strong with "Hinv") as "Hacc"; first done.
-  iIntros "!>" (l v I) "Hl". iDestruct ("Hacc" with "Hl") as "(% & Hl & Hclose)".
-  iFrame "%∗". iIntros (w) "% Hl". iApply "Hclose"; done.
-Qed.
-
-Lemma inv_mapsto_own_acc E l v I:
-  ↑inv_heapN ⊆ E →
-  inv_heap_inv -∗ l ↦_I v ={E, E ∖ ↑inv_heapN}=∗
-    (⌜I v⌝ ∗ l ↦C v ∗ (∀ w, ⌜I w ⌝ -∗ l ↦C w ={E ∖ ↑inv_heapN, E}=∗ l ↦_I w)).
-Proof.
-  iIntros (?) "#Hinv Hl".
-  iMod (inv_mapsto_own_acc with "Hinv Hl") as "(% & Hl & Hclose)"; first done.
-  iFrame "%∗". iIntros "!>" (w) "% Hl". iApply "Hclose"; done.
-Qed.
-
-Lemma inv_mapsto_acc l I E :
-  ↑inv_heapN ⊆ E →
-  inv_heap_inv -∗ l ↦_I □ ={E, E ∖ ↑inv_heapN}=∗
-    ∃ v, ⌜I v⌝ ∗ l ↦C v ∗ (l ↦C v ={E ∖ ↑inv_heapN, E}=∗ ⌜True⌝).
-Proof.
-  iIntros (?) "#Hinv Hl".
-  iMod (inv_mapsto_acc with "Hinv Hl") as ([[v|]|]) "(% & Hl & Hclose)"; [done| |done|done].
-  iIntros "!>". iExists (v). iFrame "%∗".
-Qed.
-
-(** The usable rules for [allocN] stated in terms of the [array] proposition
-are derived in te file [array]. *)
-Lemma heap_array_to_seq_meta l vs (n : nat) :
-  length vs = n →
-  ([∗ map] l' ↦ _ ∈ heap_array l vs, meta_token l' ⊤) -∗
-  [∗ list] i ∈ seq 0 n, meta_token (l +ₗ (i : nat)) ⊤.
-Proof.
-  iIntros (<-) "Hvs". iInduction vs as [|v vs] "IH" forall (l)=> //=.
-  rewrite big_opM_union; last first.
-  { apply map_disjoint_spec=> l' v1 v2 /lookup_singleton_Some [-> _].
-    intros (j&?&Hjl&?)%heap_array_lookup.
-    rewrite loc_add_assoc -{1}[l']loc_add_0 in Hjl. simplify_eq; lia. }
-  rewrite loc_add_0 -fmap_S_seq big_sepL_fmap.
-  setoid_rewrite Nat2Z.inj_succ. setoid_rewrite <-Z.add_1_l.
-  setoid_rewrite <-loc_add_assoc.
-  rewrite big_opM_singleton; iDestruct "Hvs" as "[$ Hvs]". by iApply "IH".
-Qed.
-
-Lemma heap_array_to_seq_mapsto l (v:heap_cell) (n : nat) :
-  ([∗ map] l' ↦ ov ∈ heap_array l (replicate n v), gen_heap.mapsto l' (DfracOwn 1) ov) -∗
-  [∗ list] i ∈ seq 0 n, (l +ₗ (i : nat)) O↦ v.
-Proof.
-  iIntros "Hvs". iInduction n as [|n] "IH" forall (l); simpl.
-  { done. }
-  rewrite big_opM_union; last first.
-  { apply map_disjoint_spec=> l' v1 v2 /lookup_singleton_Some [-> _].
-    intros (j&?&Hjl&_)%heap_array_lookup.
-    rewrite loc_add_assoc -{1}[l']loc_add_0 in Hjl. simplify_eq; lia. }
-  rewrite loc_add_0 -fmap_S_seq big_sepL_fmap.
-  setoid_rewrite Nat2Z.inj_succ. setoid_rewrite <-Z.add_1_l.
-  setoid_rewrite <-loc_add_assoc.
-  rewrite big_opM_singleton; iDestruct "Hvs" as "[$ Hvs]". by iApply "IH".
-Qed.
-
 Lemma wp_Malloc_seq E n :
   (0 < n)%Z →
   {{{ True }}} Malloc (Val $ LitV $ LitInt $ n) @ p; E
@@ -298,7 +66,7 @@ Proof.
 Qed.
 
 Lemma wp_free s E l (v:option val) :
-  {{{ ▷ l O↦ Some v}}} Free (Val $ LitV $ LitLoc l) (Val $ LitV $ LitInt 1) @ s; E
+  {{{ ▷ l O↦C (Some v) }}} Free (Val $ LitV $ LitLoc l) (Val $ LitV $ LitInt 1) @ s; E
   {{{ RET LitV LitUnit; True }}}.
 Proof.
   iIntros (Φ) ">Hl HΦ". iApply (wp_step with "HΦ"). iApply wp_lift_atomic_head_step; first done.
@@ -325,7 +93,7 @@ Proof.
 Qed.
 
 Lemma wp_store s E l (v':option val) v :
-  {{{ ▷ l O↦ Some v' }}} Store (Val $ LitV $ LitLoc l) (Val v) @ s; E
+  {{{ ▷ l O↦C Some v' }}} Store (Val $ LitV $ LitLoc l) (Val v) @ s; E
   {{{ RET LitV LitUnit; l ↦C v }}}.
 Proof.
   iIntros (Φ) "> Hl HΦ". iApply (wp_step with "HΦ"). iApply wp_lift_atomic_head_step; first done.
