theories/c_interface/defs.v
@@ -1,0 +1,113 @@
+From stdpp Require Export binders strings countable gmap.
+From iris.algebra Require Export ofe.
+From iris.heap_lang Require Export locations.
+From iris.prelude Require Import options.
+
+Declare Scope val_scope.
+Delimit Scope val_scope with V.
+
+Module C_intf.
+
+(** C values *)
+
+Inductive base_lit : Set :=
+  | LitInt (n : Z) | LitLoc (l : loc) | LitFunPtr (x : string).
+Inductive val :=
+  | LitV (l : base_lit).
+
+Bind Scope val_scope with C_intf.val.
+
+Global Instance base_lit_eq_dec : EqDecision base_lit.
+Proof. solve_decision. Defined.
+Global Instance val_eq_dec : EqDecision val.
+Proof. solve_decision. Defined.
+
+Global Instance base_lit_countable : Countable base_lit.
+Proof.
+ refine (inj_countable' (λ l, match l with
+  | LitInt n => (inl (inl n))
+  | LitLoc l => (inl (inr l))
+  | LitFunPtr p => (inr p)
+  end) (λ l, match l with
+  | inl (inl n) => LitInt n
+  | inl (inr l) => LitLoc l
+  | inr p => LitFunPtr p
+  end) _); by intros [].
+Qed.
+Global Instance val_countable : Countable val.
+Proof.
+  set (enc := fun e => match e with LitV l => l end).
+  set (dec := LitV).
+  refine (inj_countable' enc dec _).
+  by intros [].
+Qed.
+
+Global Instance val_inhabited : Inhabited val := populate (LitV (LitInt 0)).
+Canonical Structure valO := leibnizO val.
+
+Definition LitBool (b : bool) : base_lit := LitInt (if b then 1%Z else 0%Z).
+Definition LitUnit : base_lit := LitInt 0.
+
+(** C state *)
+
+Notation heap_cell := (option (option val)).
+Notation Deallocated := (None : heap_cell).
+Notation Uninitialized := (Some None : heap_cell).
+Notation Storing v := (Some (Some v) : heap_cell).
+
+(** The state: heaps of heap_cells. *)
+Notation c_state := (gmap loc (option (option val))).
+
+Global Instance state_inhabited : Inhabited c_state :=
+  populate inhabitant.
+
+Canonical Structure stateO := leibnizO c_state.
+
+(* Contiguous regions in the heap, i.e. arrays *)
+
+Definition state_upd_heap (f: gmap loc heap_cell → gmap loc heap_cell) (σ: c_state) : c_state :=
+  f σ.
+Global Arguments state_upd_heap _ !_ /.
+
+Fixpoint heap_array (l : loc) (vs : list heap_cell) : gmap loc heap_cell :=
+  match vs with
+  | [] => ∅
+  | v :: vs' => {[l := v]} ∪ heap_array (l +ₗ 1) vs'
+  end.
+
+Lemma heap_array_singleton l v : heap_array l [v] = {[l := v]}.
+Proof. by rewrite /heap_array right_id. Qed.
+
+Lemma heap_array_lookup l vs ow k :
+  heap_array l vs !! k = Some ow ↔
+  ∃ j, (0 ≤ j)%Z ∧ k = l +ₗ j ∧ vs !! (Z.to_nat j) = Some ow.
+Proof.
+  revert k l; induction vs as [|v' vs IH]=> l' l /=.
+  { rewrite lookup_empty. naive_solver lia. }
+  rewrite -insert_union_singleton_l lookup_insert_Some IH. split.
+  - intros [[-> ?] | (Hl & j  & ? & -> & ?)].
+    { eexists 0. rewrite loc_add_0. naive_solver lia. }
+    eexists (1 + j)%Z. rewrite loc_add_assoc !Z.add_1_l Z2Nat.inj_succ; auto with lia.
+  - intros (j & w & -> & Hil). destruct (decide (j = 0)); simplify_eq/=.
+    { rewrite loc_add_0; eauto. }
+    right. split.
+    { rewrite -{1}(loc_add_0 l). intros ?%(inj (loc_add _)); lia. }
+    assert (Z.to_nat j = S (Z.to_nat (j - 1))) as Hj.
+    { rewrite -Z2Nat.inj_succ; last lia. f_equal; lia. }
+    rewrite Hj /= in Hil.
+    eexists (j - 1)%Z. rewrite loc_add_assoc Z.add_sub_assoc Z.add_simpl_l.
+    auto with lia.
+Qed.
+
+Lemma heap_array_map_disjoint (h : gmap loc heap_cell) (l : loc) (vs : list _) :
+  (∀ i, (0 ≤ i)%Z → (i < length vs)%Z → h !! (l +ₗ i) = None) →
+  (heap_array l vs) ##ₘ h.
+Proof.
+  intros Hdisj. apply map_disjoint_spec=> l' v1 v2.
+  intros (j&w&->&Hj%lookup_lt_Some%inj_lt)%heap_array_lookup.
+  move: Hj. rewrite Z2Nat.id // => ?. by rewrite Hdisj.
+Qed.
+
+End C_intf.
+
+Export C_intf.
