theories/c_interface/notation.v
@@ -1,0 +1,11 @@
+From melocoton.c_interface Require Export defs.
+From iris.prelude Require Import options.
+
+(** Coercions to make programs easier to type. *)
+Coercion LitInt : Z >-> base_lit.
+Coercion LitBool : bool >-> base_lit.
+Coercion LitLoc : loc >-> base_lit.
+
+(* No scope, does not conflict and scope is often not inferred properly. *)
+Notation "# l" := (LitV l%Z%V%stdpp) (at level 8, format "# l").
+Notation "& f" := (LitV (LitFunPtr f)) (at level 8, format "& f").
