theories/c_interface/pretty.v
@@ -1,0 +1,21 @@
+From stdpp Require Export pretty.
+From melocoton.c_interface Require Import defs.
+From iris.prelude Require Import options.
+
+(** * Pretty printing for C values *)
+
+Global Instance pretty_loc : Pretty loc :=
+  λ l, pretty l.(loc_car).
+
+Global Instance pretty_base_lit : Pretty base_lit :=
+  λ l, match l with
+       | LitInt z => pretty z
+       | LitLoc l => "(loc " +:+ pretty l +:+ ")"
+       | LitFunPtr p => "(& " +:+ p +:+ ")"
+       end.
+
+Global Instance pretty_val : Pretty val :=
+  fix go v :=
+    match v with
+    | LitV l => pretty l
+    end.
