theories/c_interop/laws.v
@@ -1,0 +1,46 @@
+From iris.proofmode Require Import proofmode.
+From melocoton.interop Require Import basics basics_resources weakestpre wp_update_laws.
+From melocoton.ml_lang Require Import primitive_laws.
+From melocoton.c_interface Require Export resources.
+From melocoton.c_lang Require Import primitive_laws tactics notation proofmode.
+From iris.prelude Require Import options.
+
+(* Derived laws for C<->ML interop.
+
+   These follow from the generic rules of the wrapper (in interop/) that work
+   for any language obeying the C interface (c_interface/) -- specialized to our
+   concrete C language (c_lang/). *)
+
+Section Laws.
+
+Context {hlc : has_lc}.
+Context {Σ : gFunctors}.
+Context `{!heapGS_ML Σ, !heapGS_C Σ, !invGS_gen hlc Σ}.
+Context `{!wrapperGS Σ}.
+
+Lemma store_to_root E pe (l:loc) (v v' : lval) w θ :
+  repr_lval θ v w →
+  {{{ GC θ ∗ l ↦roots v' }}}
+     (#l <- w)%E @ pe; E
+  {{{ RET LitV LitUnit; GC θ ∗ l ↦roots v }}}.
+Proof.
+  iIntros (Hrepr Φ) "(HGC&Hroot) HΦ".
+  iDestruct (update_root with "[$HGC $Hroot]") as (w') "(Hpto & _ & Hupd)".
+  iApply wp_fupd.
+  iApply (wp_store with "Hpto"). iIntros "!> Hpto".
+  iMod ("Hupd" with "[$Hpto]") as "(? & ?)"; first done.
+  iApply "HΦ". by iFrame.
+Qed.
+
+Lemma load_from_root E pe (l:loc) (v : lval) dq θ :
+  {{{ GC θ ∗ l ↦roots{dq} v }}}
+     ( * #l)%E @ pe; E
+  {{{ w, RET w; l ↦roots{dq} v ∗ GC θ ∗ ⌜repr_lval θ v w⌝ }}}.
+Proof.
+  iIntros (Φ) "(HGC&Hroot) HΦ".
+  iDestruct (access_root with "[$HGC $Hroot]") as (w') "(Hpto & %Hrepr & Hupd)".
+  iApply (wp_load with "Hpto"). iIntros "!> Hpto".
+  iDestruct ("Hupd" with "Hpto") as "(?&?)". iApply "HΦ". by iFrame.
+Qed.
+
+End Laws.
