theories/c_lang/notation.v
@@ -1,11 +1,8 @@
+From melocoton.c_interface Require Export notation.
 From melocoton.c_lang Require Export lang.
 From iris.prelude Require Import options.
 
 (** Coercions to make programs easier to type. *)
-Coercion LitInt : Z >-> base_lit.
-Coercion LitBool : bool >-> base_lit.
-Coercion LitLoc : loc >-> base_lit.
-
 Coercion Val : val >-> expr.
 Coercion Var : string >-> expr.
 
@@ -16,11 +13,6 @@ Notation SeqCtx e2 := (LetCtx BAnon e2) (only parsing).
 (* Skip should be atomic, we sometimes open invariants around
    it. Hence, we need to explicitly use LamV instead of e.g., Seq. *)
 Notation Skip := (Seq (Val $ LitV LitUnit) (Val $ LitV LitUnit)).
-
-(* No scope for the values, does not conflict and scope is often not inferred
-properly. *)
-Notation "# l" := (LitV l%Z%V%stdpp) (at level 8, format "# l").
-Notation "& f" := (LitV (LitFunPtr f)) (at level 8, format "& f").
 
 Notation "* e" := (Load e%E) (at level 9, right associativity) : expr_scope.
 Notation "'malloc' '(' e ')'" := (Malloc e%E) (at level 10) : expr_scope.
