theories/c_lang/pretty.v
@@ -1,33 +1,13 @@
 From stdpp Require Export pretty.
-
+From melocoton.c_interface Require Export pretty.
 From melocoton.c_lang Require Import lang.
 From iris.prelude Require Import options.
-
-(** * Pretty printing for HeapLang values *)
-
-Global Instance pretty_loc : Pretty loc :=
-  λ l, pretty l.(loc_car).
-
-Global Instance pretty_base_lit : Pretty base_lit :=
-  λ l, match l with
-       | LitInt z => pretty z
-       | LitLoc l => "(loc " +:+ pretty l +:+ ")"
-       | LitFunPtr p => "(& " +:+ p +:+ ")"
-       end.
 
 Global Instance pretty_binder : Pretty binder :=
   λ b, match b with
        | BNamed x => x
        | BAnon => "<>"
        end.
-
-(** Note that this instance does not print function bodies and is thus not
-injective (unlike most `pretty` instances). *)
-Global Instance pretty_val : Pretty val :=
-  fix go v :=
-    match v with
-    | LitV l => pretty l
-    end.
 
 Global Instance pretty_un_op : Pretty un_op :=
   λ op, match op with
