theories/interop/wp_simulation.v
@@ -7,9 +7,9 @@ From melocoton.mlanguage Require Import weakestpre.
 From melocoton.interop Require Import state lang basics_resources.
 From iris.base_logic.lib Require Import ghost_map ghost_var.
 From iris.proofmode Require Import proofmode.
-From melocoton.c_lang Require Import lang lang_instantiation primitive_laws.
+From melocoton.c_interface Require Import defs resources.
 From melocoton.ml_lang Require Import lang lang_instantiation primitive_laws.
-From melocoton.interop Require Import basics prims weakestpre wp_block_sim
+From melocoton.interop Require Import basics basics_resources prims weakestpre wp_block_sim
   wp_utils wp_ext_call_laws wp_boundary_laws.
 Import Wrap.
 
@@ -20,9 +20,6 @@ Context {Σ : gFunctors}.
 Context `{!heapGS_ML Σ, !heapGS_C Σ}.
 Context `{!invGS_gen hlc Σ}.
 Context `{!wrapperGS Σ}.
-
-Notation MLval := ML_lang.val.
-Notation Cval := C_lang.val.
 
 Implicit Types P : iProp Σ.
 Import mlanguage.
